tests/bug-reports/closed/Bug2057.fst
@@ -1,38 +1,18 @@
 module Bug2057
 
-type unit : Type = unit
+type repr (a:Type) = a
 
-type repr (a:Type) (_:unit) = a
+let return (a:Type) (x:a) : repr a = x
+let bind (a:Type) (b:Type) (f:repr a) (g:a -> repr b) : repr b = g f
 
-let return (a:Type) (x:a) : repr a () = x
-let bind (a:Type) (b:Type) (f:repr a ()) (g:a -> repr b ()) : repr b () = g f
-
-layered_effect {
-  M : Type -> unit -> Effect
-  with repr = repr;
-       return = return;
-       bind = bind
+effect {
+  M with { repr; return; bind }
 }
 
-let lift_PURE_M (a:Type) (wp:pure_wp a) (f:unit -> PURE a wp)
-  : Pure (repr a ()) (requires wp (fun _ -> True)) (ensures fun _ -> True)
-  = FStar.Monotonic.Pure.elim_pure_wp_monotonicity wp;
-    f ()
+let lift_PURE_M (a:Type) (f:unit -> a) : repr a = f ()
 
 sub_effect PURE ~> M = lift_PURE_M
 
-assume val f (_:unit) : M int ()
+assume val f (_:unit) : M int
 
-(*
- * Expected type "Effect"; but "Bug2057.M Prims.int" has type "_: Bug2057.unit -> Prims.Tot Effect"
- *)
-[@@ expect_failure [12]]
 let g () : M int = f ()
-
-(*
- * Example from #1861
- *)
-
-[@@expect_failure [12]]
-let test : (f : unit -> Exn unit _ _) -> unit =
-    fun (f : unit -> Exn unit) -> ()
