tests/tactics/InspectEffComp.fst
@@ -2,17 +2,16 @@ module InspectEffComp
 
 open FStar.Tactics.V2
 
-open FStar.Monotonic.Pure
-
 let test () : Type0 =
   _ by
-    (let t = (`(int -> PURE int (as_pure_wp (fun p -> p 42)))) in
+    (let t = (`(int -> PURE int (requires True) (ensures fun r -> r == 42))) in
      match inspect t with
      | Tv_Arrow bv c ->
        let c' =
          begin match inspect_comp c with
          | C_Eff us eff res args decrs ->
-                 let args' = [(`(as_pure_wp (fun p -> p 17)), Q_Explicit)] in
+                 let args' = [(`(True), Q_Explicit);
+                              (`(fun (r:int) -> r == 17), Q_Explicit)] in
                  pack_comp (C_Eff us eff res args' decrs)
          | _ -> fail "no"
          end
@@ -22,4 +21,4 @@ let test () : Type0 =
      | _ -> fail "impossible")
 
 
-let _ = assert (test () == (int -> PURE int (as_pure_wp (fun p -> p 17))))
+let _ = assert (test () == (int -> PURE int (requires True) (ensures fun r -> r == 17)))
