simple-lib/FStar.Prelude.fsti
@@ -1,0 +1,7 @@
+[@@"no_prelude"]
+module FStar.Prelude
+
+include Prims
+include FStar.Pervasives.Native
+include FStar.Pervasives
+include FStar.Attributes
