simple-lib/Prims.fst
@@ -1,0 +1,525 @@
+(*
+   Copyright 2008-2020 Microsoft Research
+
+   Licensed under the Apache License, Version 2.0 (the "License");
+   you may not use this file except in compliance with the License.
+   You may obtain a copy of the License at
+
+       http://www.apache.org/licenses/LICENSE-2.0
+
+   Unless required by applicable law or agreed to in writing, software
+   distributed under the License is distributed on an "AS IS" BASIS,
+   WITHOUT WARRANTIES OR CONDITIONS OF ANY KIND, either express or implied.
+   See the License for the specific language governing permissions and
+   limitations under the License.
+*)
+[@@"no_prelude"]
+module Prims
+
+/// This module is implicitly opened in the scope of all other modules.
+///
+/// It provides the very basic primitives on which F* is
+/// built, including the definition of total functions, the basic
+/// logical connectives, the PURE and GHOST effects and the like.
+///
+/// While some of the primitives have logical significance, others are
+/// define various conveniences in the language, e.g., type of
+/// attributes.
+
+
+(***** Begin trusted primitives *****)
+
+(** Primitives up to the definition of the GTot effect are trusted
+    Beyond that all definitions are fully verified *)
+
+
+
+(** Type of attributes *)
+assume new
+type attribute : Type0 
+
+
+(** This attribute marks definitions for logical connectives that should
+    not be unfolded during tactics. *)
+assume
+val tac_opaque : attribute
+
+(** This attribute is added to all projectors. *)
+assume
+val projector : attribute
+
+(** This attribute is added to all discriminators. *)
+assume
+val discriminator : attribute
+
+(** This attribute can be used on type binders to make unifier attempt
+    to unrefine them before instantiating them. This is useful in polymorphic
+    definitions where the type does not change the result type, for example
+    eq2 below. Using the attribute, an equality between two nats will happen
+    at type int, which is more canonical.
+
+    This feature is experimental and only enabled with "--ext __unrefine" *)
+assume
+val unrefine : attribute
+
+(** This attribute can be attached to a type definition to partly counter the
+    behavior of the `unrefine` attribute. It will cause the definition marked
+    `do_not_unrefine` to not be unfolded during the unrefining process. *)
+assume
+val do_not_unrefine : attribute
+
+(** A binder in a definition/declaration may optionally be annotated as strictly_positive
+    When the let definition is used in a data constructor type in an inductive
+    definition, this annotation is used to check the positivity of the inductive
+
+    Further F* checks that the binder is actually positive in the let definition
+
+    See tests/micro-benchmarks/Positivity.fst and NegativeTests.Positivity.fst for a few examples
+  *)
+assume val strictly_positive : attribute
+
+(** The type of propositions. *)
+assume val prop : Type0
+
+(** A predicate to express when a type supports decidable equality
+    The type-checker emits axioms for [hasEq] for each inductive type *)
+assume
+type hasEq : Type -> GTot prop
+
+(** A convenient abbreviation, [eqtype] is the type of types in
+    universe 0 which support decidable equality *)
+type eqtype = a: Type0{hasEq a}
+
+(** [bool] is a two element type with elements [true] and [false]. We
+    assume it is primitive, for convenient interop with other
+    languages, although it could easily be defined as an inductive type
+    with two cases, [BTrue | BFalse] *)
+assume new
+type bool : eqtype 
+
+(** [empty] is the empty inductive type. The type with no
+    inhabitants represents logical falsehood. Note, [empty] is
+    seldom used directly in F*. We instead use its "squashed" variant,
+    [False], see below. *)
+type empty = 
+
+(** [trivial] is the singleton inductive type---it is trivially
+    inhabited. Like [empty], [trivial] is seldom used. We instead use
+    its "squashed" variants, [True] *)
+type trivial = | T
+
+(** [unit]: another singleton type, with its only inhabitant written [()]
+    we assume it is primitive, for convenient interop with other languages *)
+assume new
+type unit : eqtype
+
+(** [squash p] is a central type in F*---[squash p] is the proof
+    irrelevant analog of [p] and is represented as a unit
+    refinement. Squashed proofs are typically discharged using an SMT
+    solver, without any proof terms explicitly reconstructed. As
+    such, one way to think of [squash p] is as the type of properties
+    proven using classical axioms without building proof terms.
+
+    Note, [squash p] is just a unit refinement, it resides in universe
+    0, lowering the universe of [p]. From this perspective, one may
+    also see [squash] as a coercion down to universe 0.
+
+    The type is marked [tac_opaque] to indicate to Meta-F* that
+    instances of [squash] should not be unfolded when evaluating
+    tactics (since many optimizations in F*'s SMT encoding rely
+    specifically on occurrences of [squash].
+
+    See FStar.Squash for various ways of manipulating squashed
+    types. *)
+[@@ tac_opaque]
+type squash (p: prop) : Type0 = x: unit{p}
+
+(** An attribute indicating that a symbol is an smt theory symbol and
+    hence may not be used in smt patterns.  The typechecker warns if
+    such symbols are used in patterns *)
+assume
+val smt_theory_symbol:attribute
+
+(** Written with the `True` syntax, `l_True` is the true proposition. *)
+[@@ smt_theory_symbol]
+assume val l_True : prop
+
+(** Written with the `False` syntax, `l_False` is the false proposition. *)
+[@@ smt_theory_symbol]
+assume val l_False : prop
+
+(**** Effects
+
+    In this simplified effect system an effect is just a name.  A
+    computation type is [M t (requires pre) (ensures post)], where
+    [pre] is a proposition and [post] is a predicate on the result. *)
+
+total assume effect PURE
+total assume effect GHOST
+
+(** [PURE] computations can be lifted to [GHOST] (but not vice versa),
+    *)
+assume sub_effect PURE ~> GHOST
+
+(** Hoare-style abbreviations.  Effect abbreviations are parameterized
+    by the result type only; any pre/postcondition written at the use
+    site is conjoined with the one in the abbreviation. *)
+effect Pure  (a: Type) = PURE a
+effect Tot   (a: Type) = PURE a
+effect Ghost (a: Type) = GHOST a
+effect GTot  (a: Type) = GHOST a
+
+
+(** The type of provable equalities, defined as the usual inductive
+    type with a single constructor for reflexivity.  As with the other
+    connectives, we often work instead with the squashed version of
+    equality, below. *)
+type equals (#a: Type) (x: a) : a -> Type = | Refl : equals x x
+
+(** `eq2` is propositional equality, usually written with the `==` syntax. *)
+//    TODO: instead of hard-wiring the == syntax,
+//          we should just rename eq2 to op_Equals_Equals
+[@@ smt_theory_symbol]
+assume val eq2 (#[@@@unrefine] a: Type) (x: a) (y: a) : prop
+
+(** bool-to-prop coercion: This is often automatically inserted type,
+    when using a boolean in context expecting a type. But,
+    occasionally, one may have to write [b2t] explicitly *)
+let b2t (b: bool) : prop = (b == true)
+
+(** constructive conjunction *)
+type pair (p: Type) (q: Type) = | Pair : _1:p -> _2:q -> pair p q
+
+(** Written with the `/\` syntax, `l_and` is the propositional conjunction. *)
+[@@ smt_theory_symbol]
+assume val l_and ([@@@strictly_positive] p: prop) ([@@@strictly_positive] q: prop) : prop
+
+(** constructive disjunction *)
+type sum (p: Type) (q: Type) =
+  | Left : v:p -> sum p q
+  | Right : v:q -> sum p q
+
+(** Written with the `\/` syntax, `l_or` is the propositional disjunction. *)
+[@@ smt_theory_symbol]
+assume val l_or ([@@@strictly_positive] p: prop) ([@@@strictly_positive] q: prop) : prop
+
+(** Written with the `==>` syntax, `l_imp` is the propositional implication.
+    Note, [==>] binds weaker than [/\] and [\/] *)
+[@@ smt_theory_symbol]
+assume val l_imp (p: prop) ([@@@strictly_positive] q: prop) : prop
+
+(** double implication, infix binary [<==>] *)
+[@@ smt_theory_symbol]
+let l_iff (p: prop) (q: prop) : prop = (p ==> q) /\ (q ==> p)
+
+(** negation, prefix unary [~] *)
+[@@ smt_theory_symbol]
+type l_not (p: prop) : prop = p ==> False
+
+(** l_ITE is a form of if-then-else at the level of
+    propositions. It's not used much.
+
+    TODO: Can we remove it *)
+unfold
+let l_ITE (p: prop) (q: prop) (r: prop) : prop = (p ==> q) /\ (~p ==> r)
+
+(** One of the main axioms provided by prims is [precedes], a
+    built-in well-founded partial order over all terms. It's typically
+    written with an infix binary [<<].
+
+    The [<<] order includes:
+        * The [<] ordering on natural numbers
+        * The subterm ordering on inductive types
+        * [f x << D f] for data constructors D of an inductive t whose
+          arguments include a ghost or total function returning a t *)
+
+assume
+type precedes : #a: Type -> #b: Type -> a -> b -> prop
+
+(** The type of primitive strings of characters; See FStar.String *)
+assume new
+type string : eqtype 
+
+(** This attribute can be added to the declaration or definition of
+    any top-level symbol. It causes F* to report a warning on any
+    use of that symbol, printing the [msg] argument.
+    
+    This is used, for instance to:
+    
+    - tag every escape hatch, e.g., [assume], [admit], etc
+
+    Reports for uses of symbols tagged with this attribute
+    are controlled using the `--report_assumes` option
+    and warning number 334. 
+    
+    See tests/micro-benchmarks/WarnOnUse.fst
+ *)
+assume
+val warn_on_use (msg: string) : Tot unit
+
+(** The [deprecated "s"] attribute: "s" is an alternative function
+    that should be printed in the warning it can be omitted if the use
+    case has no such function *)
+assume
+val deprecated (s: string) : Tot unit
+
+
+(** Within the SMT encoding, we have a relation [(HasType e t)]
+    asserting that (the encoding of) [e] has a type corresponding to
+    (the encoding of) [t].
+
+    It is sometimes convenient, e.g., when writing triggers for
+    quantifiers, to have access to this relation at the source
+    level. The [has_type] predicate below reflects the SMT encodings
+    [HasType] relation. We also use it to define the type [prop] or
+    proof irrelevant propositions, below.
+
+    Note, unless you have a really good reason, you probably don't
+    want to use this [has_type] predicate. F*'s type theory certainly
+    does not internalize its own typing judgment *)
+[@@deprecated "'has_type' is intended for internal use and debugging purposes only; \
+                do not rely on it for your proofs"]
+assume
+type has_type : #a: Type -> a -> Type -> prop 
+
+(** Universal quantification, written [forall (x:a). p x] *)
+[@@ tac_opaque; smt_theory_symbol]
+assume val l_Forall (#a: Type) ([@@@strictly_positive] p: (a -> GTot prop)) : prop
+
+#push-options "--warn_error -288" 
+(** [p1 `subtype_of` p2] when every element of [p1] is also an element
+    of [p2]. *)
+let subtype_of (p1 p2: Type) = forall (x: p1). has_type x p2
+#pop-options
+
+(**** Escape hatches *)
+
+(** [Admit] discards the verification condition of its continuation *)
+effect Admit (a: Type) = PURE a (ensures (fun _ -> l_False))
+
+(***** End trusted primitives *****)
+
+
+(** This point onward, F* fully verifies all the definitions *)
+
+(** [===] heterogeneous equality *)
+let ( === ) (#a #b: Type) (x: a) (y: b) : prop = a == b /\ x == y
+
+(** Dependent pairs [dtuple2] in concrete syntax is [x:a & b x].
+    Its values can be constructed with the concrete syntax [(| x, y |)] *)
+unopteq
+type dtuple2 (a: Type) (b: (a -> GTot Type)) =
+  | Mkdtuple2 : _1: a -> _2: b _1 -> dtuple2 a b
+
+(** Squashed existential quantification, or dependent sums,
+    are written [exists (x:a). p x] : specialized to Type0 *)
+[@@ smt_theory_symbol]
+assume val l_Exists (#a: Type) ([@@@strictly_positive] p: (a -> GTot prop)) : prop
+
+(** Primitive type of mathematical integers, mapped to zarith in OCaml
+    extraction and to the SMT sort of integers *)
+assume new
+type int : eqtype 
+
+(**** Basic operators on booleans and integers *)
+
+(** [&&] boolean conjunction *)
+
+[@@ smt_theory_symbol]
+assume
+val op_AmpAmp: bool -> bool -> Tot bool
+
+(** [||] boolean disjunction *)
+
+[@@ smt_theory_symbol]
+assume
+val op_BarBar: bool -> bool -> Tot bool
+
+(** [not] boolean negation *)
+
+[@@ smt_theory_symbol]
+assume
+val op_Negation: bool -> Tot bool
+
+(** [*] integer multiplication *)
+
+[@@ smt_theory_symbol]
+assume
+val op_Star: int -> int -> Tot int
+
+(** [-] integer subtraction *)
+
+[@@ smt_theory_symbol]
+assume
+val op_Subtraction: int -> int -> Tot int
+
+(** [+] integer addition *)
+
+[@@ smt_theory_symbol]
+assume
+val op_Addition: int -> int -> Tot int
+
+(** [-] prefix unary integer negation *)
+
+[@@ smt_theory_symbol]
+assume
+val op_Minus: int -> Tot int
+
+(** [<=] integer comparison *)
+
+[@@ smt_theory_symbol]
+assume
+val op_LessThanOrEqual: int -> int -> Tot bool
+
+(** [>] integer comparison *)
+
+[@@ smt_theory_symbol]
+assume
+val op_GreaterThan: int -> int -> Tot bool
+
+(** [>=] integer comparison *)
+
+[@@ smt_theory_symbol]
+assume
+val op_GreaterThanOrEqual: int -> int -> Tot bool
+
+(** [<] integer comparison *)
+
+[@@ smt_theory_symbol]
+assume
+val op_LessThan: int -> int -> Tot bool
+
+(** [=] decidable equality on [eqtype] *)
+
+[@@ smt_theory_symbol]
+assume
+val op_Equality: #[@@@unrefine]a: eqtype -> a -> a -> Tot bool
+
+(** [<>] decidable dis-equality on [eqtype] *)
+
+[@@ smt_theory_symbol]
+assume
+val op_disEquality: #[@@@unrefine]a: eqtype -> a -> a -> Tot bool
+
+(** The extensible open inductive type of exceptions *)
+assume new
+type exn : Type0 
+
+(** String concatenation and its abbreviation as [^].  TODO, both
+    should be removed in favor of what is present in FStar.String *)
+assume
+val strcat: string -> string -> Tot string
+inline_for_extraction unfold
+let op_Hat s1 s2 = strcat s1 s2
+
+(** The inductive type of polymorphic lists *)
+type list (a: Type) =
+  | Nil : list a
+  | Cons : hd: a -> tl: list a -> list a
+
+(** The keyword term-level keyword [assume] is desugared to [_assume].
+    It explicitly provides an escape hatch to assume a given property
+    [p]. *)
+[@@ warn_on_use "Uses an axiom"]
+assume
+val _assume (p: prop) : Pure unit (requires (True)) (ensures (fun x -> p))
+
+(** [admit] is another escape hatch: It discards the continuation and
+    returns a value of any type *)
+[@@ warn_on_use "Uses an axiom"]
+assume
+val admit: #a: Type -> unit -> Admit a
+
+(** [magic] is another escape hatch: It retains the continuation but
+    returns a value of any type *)
+[@@ warn_on_use "Uses an axiom"]
+assume
+val magic: #a: Type -> unit -> Tot a
+
+(** [unsafe_coerce] is another escape hatch: It coerces an [a] to a
+    [b].  *)
+[@@ warn_on_use "Uses an axiom"]
+irreducible
+let unsafe_coerce (#a #b: Type) (x: a) : b =
+  admit ();
+  x
+
+(** The keyword term-level keyword [assert] is desugared to [_assert].
+    It force a proof of a property [p], then assuming [p] for the
+    continuation. *)
+val _assert (p: prop) : Pure unit (requires p) (ensures (fun x -> p))
+let _assert p = ()
+
+(** Logically equivalent to assert; TODO remove? *)
+val cut (p: prop) : Pure unit (requires p) (fun x -> p)
+let cut p = ()
+
+(** Indefinite description is an axiom that allows picking a witness for an existential quantifier
+
+For some background on the axiom, see:
+  https://github.com/coq/coq/wiki/CoqAndAxioms#indefinite-description--hilberts-epsilon-operator
+  https://en.wikipedia.org/wiki/Theory_of_descriptions#Indefinite_descriptions *)
+assume val indefinite_description (#a: Type) (p: (a -> prop) { exists x. p x })
+  : GTot (x: a { p x })
+
+(* prop-to-bool coercion.
+
+   [t2b_pred] is a top-level definition rather than a local one on purpose: the
+   witness for [indefinite_description]'s existential is found by instantiating
+   it with the applications appearing in the assertion below, which only works
+   as long as they survive as applications. *)
+let t2b_pred (p: prop) (b: bool) : prop = b <==> p
+
+irreducible let t2b (p: prop) : GTot (b:bool { b <==> p }) =
+  assert t2b_pred p true \/ t2b_pred p false;
+  indefinite_description (t2b_pred p)
+
+(** The type of non-negative integers *)
+type nat = i: int{i >= 0}
+
+(** The type of positive integers *)
+type pos = i: int{i > 0}
+
+(** The type of non-zero integers *)
+type nonzero = i: int{i <> 0}
+
+/// Arbitrary precision ints are compiled to zarith (big_ints) in
+/// OCaml and to .NET BigInteger in F#. Both the modulus and division
+/// operations are Euclidean and are mapped to the corresponding
+/// theory symbols in the SMT encoding
+
+(** Euclidean modulus *)
+
+[@@ smt_theory_symbol]
+assume
+val op_Modulus: int -> nonzero -> Tot int
+
+(** Euclidean division, written [/] *)
+
+[@@ smt_theory_symbol]
+assume
+val op_Division: int -> nonzero -> Tot int
+
+(** [pow2 x] is [2^x]:
+
+    TODO: maybe move this to FStar.Int *)
+let rec pow2 (x: nat) : Tot pos =
+  match x with
+  | 0 -> 1
+  | _ -> 2 * pow2 (x - 1)
+
+(** [min] computes the minimum of two [int]s *)
+let min x y = if x <= y then x else y
+
+(** [abs] computes the absolute value of an [int] *)
+let abs (x: int) : Tot int = if x >= 0 then x else - x
+
+(** A primitive printer for booleans:
+
+    TODO: unnecessary, this could easily be defined *)
+assume
+val string_of_bool: bool -> Tot string
+
+(** A primitive printer for [int] *)
+assume
+val string_of_int: int -> Tot string
